src/Refinements/CowZonedDiskRefinesBlockDisk.dfy
@@ -1,0 +1,66 @@
+include "../Utils.dfy"
+include "../Types.dfy"
+include "../Disks/BlockDisk.dfy"
+include "../Disks/CowZonedDisk.dfy"
+
+module CowZonedDiskRefinesBlockDisk {
+    import opened NativeTypes
+    import opened Types
+    import opened Utils
+    import opened Zone
+
+    import C = CowZonedDisk
+    import A = BlockDisk
+
+    // wow what a great name
+    lemma FlattenedSeqOfEqualLengthedSeqLengthLemma<T>(s: seq<seq<T>>)
+        requires |s| > 0
+        requires forall i,j :: 0 <= i < j < |s| ==> |s[i]| == |s[j]|
+        ensures |Flatten(s)| == |s| * |s[0]|
+    {}
+
+    function IC(c: C.Constants): A.Constants
+        requires C.ConstantsValid(c)
+        ensures A.ConstantsValid(IC(c))
+    {
+        // A CowZonedDisk can be modeled as an abstract block disk, 
+        // with the buffer zone "invisible" to the outside world.
+        A.Constants(
+            C.BlocksPerZone(c) as int * (|c.zd.zone_map| - 1)
+        )
+    }
+
+    function I(c: C.Constants, s: C.State): A.State
+        requires C.Valid(c,s)
+        ensures A.Valid(IC(c), I(c, s))
+    {
+        var buffer_zone := s.buffer_zone;
+        var zones: seq<Zone.State> := 
+            s.zd.zones[0..buffer_zone] + s.zd.zones[buffer_zone + 1..];
+
+        assert |zones| == |s.zd.zones| - 1;
+        
+        var ssblocks: seq<seq<Block.State>> := seq(|zones|, z requires 0 <= z < |zones| => zones[z].blocks);
+        assert forall i,j :: 0 <= i < j < |ssblocks| ==> |ssblocks[i]| == |ssblocks[j]|;
+
+        var blocks : seq<Block.State> := Flatten(ssblocks);
+
+        FlattenedSeqOfEqualLengthedSeqLengthLemma(ssblocks);
+
+        // XXX: We don't know that, even though all the Blocks in the seq<seq<Block>> were valid, that
+        // after flattening they remain exactly the same.  Punch a hole in the proof with an assume until
+        // I can figure out why this might be.
+        assert forall i,j :: 0 <= i < |ssblocks| ==> 0 <= j < |zones[i].blocks| 
+            ==> Block.Valid(ssblocks[i][j]);
+        assume forall i :: 0 <= i < |blocks| ==> Block.Valid(blocks[i]);
+
+        A.State(blocks)
+    }
+
+
+    lemma RefinesInit(c: C.Constants)
+        requires C.ConstantsValid(c)
+        requires C.Valid(c, C.Init(c))
+        ensures A.Valid(IC(c), I(c, C.Init(c)))
+    {}
+}
