src/Utils.dfy
@@ -26,6 +26,33 @@ module Utils {
         ss[0] + Flatten(ss[1..])
     }
 
+    // Needed for CowZonedDiskRefinesBlockDisk::I
+    lemma FlattenedContentsUnchanged<T>(ss: seq<seq<T>>, s: seq<T>)
+        requires Flatten(ss) == s
+        ensures forall i, j :: 
+            0 <= i < |ss| ==> 0 <= j < |ss[i]| ==>
+                exists k :: 0 <= k < |s| && s[k] == ss[i][j]
+    {
+        if |ss| == 0 {}
+        else {
+            var hd: seq<T> := ss[0];
+            var hdlen := |ss[0]|;
+            var tl: seq<seq<T>> := ss[1..];
+
+            assert forall i :: 0 <= i < hdlen ==> hd[i] in s;
+            FlattenedContentsUnchanged(tl, s[hdlen..]);
+        }
+    }
+
+    /*
+    lemma FlattenedContentsUnchanged<T>(ss: seq<seq<T>>, s: seq<T>)
+        requires Flatten(ss) == s
+        ensures (set x | x in Flatten(ss)) == (set i, j | 0 <= i < |ss| && 0 <= j < |ss[i]| :: ss[i][j])
+    {
+
+    }
+    */
+
     function method Map<T,U>(f: (T ~> U), s: seq<T>) : seq<U>
         reads f.reads
         requires forall i :: 0 <= i < |s| ==> f.requires(s[i])
@@ -33,6 +60,13 @@ module Utils {
     {
         if |s| == 0 then [] else
         [f(s[0])] + Map(f, s[1..])
+    }
+
+    function method FlatMapSeq<T, U>(f: T ~> seq<U>, s: seq<T>) : seq<U>
+        reads f.reads
+        requires forall i :: 0 <= i < |s| ==> f.requires(s[i])
+    {
+        Flatten(Map(f, s))
     }
 
     function method Filter<T>(f: (T ~> bool), s: seq<T>) : seq<T>
@@ -43,4 +77,6 @@ module Utils {
         if |s| == 0 then [] else
         (if f(s[0]) then [s[0]] else []) + Filter(f, s[1..])
     }
+
+
 }
